working/composition/event_based_refinement/load_balancer/Client.v.dfy
@@ -3,14 +3,14 @@ include "AdditionServiceSpec.t.dfy"
 module ClientHost {
     import opened Types
 
-    datatype Constants = Constants(x: int, y: int)
+    datatype Constants = Constants
     {
         ghost predicate WF() {
             true
         }
     }
 
-    datatype Variables = Variables(sentRequest: bool, resp: Option<int>)
+    datatype Variables = Variables(req: Option<(int, int)>, resp: Option<int>)
     {
         ghost predicate WF(c: Constants) {
             true
@@ -18,22 +18,22 @@ module ClientHost {
     }
 
     ghost predicate Init(c: Constants, v: Variables) {
-        && !v.sentRequest
+        && v.req.None?
         && v.resp.None?
     }
 
     ghost predicate SendRequest(c: Constants, v: Variables, v': Variables, evt: Event, msgOps: MessageOps) {
-        && evt.NoOp?
+        && evt.SendRequest?
         && v.resp == v'.resp
-        && !v.sentRequest
-        && v'.sentRequest
+        && v.req.None?
+        && v'.req.Some?
         && msgOps.recv.None?
-        && msgOps.send == Some(ClientRequest(c.x, c.y))
+        && msgOps.send == Some(ClientRequest(v'.req.value.0, v'.req.value.1))
     }
 
     ghost predicate ReceiveResponse(c: Constants, v: Variables, v': Variables, evt: Event, msgOps: MessageOps) {
-        && evt.NoOp?
-        && v.sentRequest == v'.sentRequest
+        && evt.ReceiveResponse?
+        && v.req == v'.req
         && msgOps.recv.Some?
         && msgOps.recv.value.ClientResponse?
         && msgOps.send.None?
