working/composition/event_based_refinement/load_balancer/DistributedSystem.v.dfy
@@ -14,39 +14,40 @@ module DistributedSystem refines AbstractDistributedSystem {
         requires c.WF()
         ensures 0 < |behavior|
         ensures Init(c, behavior[0])
-        ensures forall i:nat | i < |behavior|-1 :: (Next(c, behavior[i], behavior[i+1], NoOp) || Next(c, behavior[i], behavior[i+1], Compute))
+        ensures forall i:nat | i < |behavior|-1 :: (Next(c, behavior[i], behavior[i+1], NoOp) || Next(c, behavior[i], behavior[i+1], SendRequest) || Next(c, behavior[i], behavior[i+1], ReceiveResponse))
         ensures behavior[|behavior|-1].WF(c)
-        ensures behavior[|behavior|-1].hosts[0].client.resp == Some(c.hosts[0].client.x + c.hosts[0].client.y)
+        ensures behavior[|behavior|-1].hosts[0].client.req.Some?
+        ensures behavior[|behavior|-1].hosts[0].client.resp == Some(behavior[|behavior|-1].hosts[0].client.req.value.0 + behavior[|behavior|-1].hosts[0].client.req.value.1)
     {
         behavior := [Variables(
             [
-                Host.ClientVariables(ClientHost.Variables(false, None)),
+                Host.ClientVariables(ClientHost.Variables(None, None)),
                 Host.ServerVariables(ServerHost.Variables(None)),
                 Host.LoadBalancerVariables(LoadBalancerHost.Variables(false, false))
             ],
             Network.Variables({})
         )];
 
-        var sent := ClientRequest(c.hosts[0].client.x, c.hosts[0].client.y);
+        var sent := ClientRequest(1, 2);
         var msgOps := MessageOps(None, Some(sent));
         behavior := behavior + [Variables(
             [
-                Host.ClientVariables(ClientHost.Variables(true, None)),
+                Host.ClientVariables(ClientHost.Variables(Some((1,2)), None)),
                 Host.ServerVariables(ServerHost.Variables(None)),
                 Host.LoadBalancerVariables(LoadBalancerHost.Variables(false, false))
             ],
             Network.Variables({ sent })
         )];
-        assert ClientHost.SendRequest(c.hosts[0].client, behavior[0].hosts[0].client, behavior[1].hosts[0].client, NoOp, msgOps);
-        assert NextStep(c, behavior[0], behavior[1], NoOp, HostActionStep(0, msgOps));
-        assert Next(c, behavior[0], behavior[1], NoOp);
+        assert ClientHost.SendRequest(c.hosts[0].client, behavior[0].hosts[0].client, behavior[1].hosts[0].client, SendRequest, msgOps);
+        assert NextStep(c, behavior[0], behavior[1], SendRequest, HostActionStep(0, msgOps));
+        assert Next(c, behavior[0], behavior[1], SendRequest);
 
         var recv := sent;
         var sent2 := LBRequest(recv.x, recv.y);
         msgOps := MessageOps(Some(recv), Some(sent2));
         behavior := behavior + [Variables(
             [
-                Host.ClientVariables(ClientHost.Variables(true, None)),
+                Host.ClientVariables(ClientHost.Variables(Some((1,2)), None)),
                 Host.ServerVariables(ServerHost.Variables(None)),
                 Host.LoadBalancerVariables(LoadBalancerHost.Variables(true, false))
             ],
@@ -62,22 +63,22 @@ module DistributedSystem refines AbstractDistributedSystem {
         msgOps := MessageOps(Some(recv2), Some(sent3));
         behavior := behavior + [Variables(
             [
-                Host.ClientVariables(ClientHost.Variables(true, None)),
+                Host.ClientVariables(ClientHost.Variables(Some((1,2)), None)),
                 Host.ServerVariables(ServerHost.Variables(Some(sum))),
                 Host.LoadBalancerVariables(LoadBalancerHost.Variables(true, false))
             ],
             Network.Variables({ sent, sent2, sent3 })
         )];
-        assert ServerHost.Compute(c.hosts[1].server, behavior[2].hosts[1].server, behavior[3].hosts[1].server, Compute, msgOps);
-        assert NextStep(c, behavior[2], behavior[3], Compute, HostActionStep(1, msgOps));
-        assert Next(c, behavior[2], behavior[3], Compute);
+        assert ServerHost.Compute(c.hosts[1].server, behavior[2].hosts[1].server, behavior[3].hosts[1].server, NoOp, msgOps);
+        assert NextStep(c, behavior[2], behavior[3], NoOp, HostActionStep(1, msgOps));
+        assert Next(c, behavior[2], behavior[3], NoOp);
 
         var recv3 := sent3;
         var sent4 := ClientResponse(recv3.sum);
         msgOps := MessageOps(Some(recv3), Some(sent4));
         behavior := behavior + [Variables(
             [
-                Host.ClientVariables(ClientHost.Variables(true, None)),
+                Host.ClientVariables(ClientHost.Variables(Some((1,2)), None)),
                 Host.ServerVariables(ServerHost.Variables(Some(sum))),
                 Host.LoadBalancerVariables(LoadBalancerHost.Variables(true, true))
             ],
@@ -91,14 +92,14 @@ module DistributedSystem refines AbstractDistributedSystem {
         msgOps := MessageOps(Some(recv4), None);
         behavior := behavior + [Variables(
             [
-                Host.ClientVariables(ClientHost.Variables(true, Some(recv4.sum))),
+                Host.ClientVariables(ClientHost.Variables(Some((1,2)), Some(recv4.sum))),
                 Host.ServerVariables(ServerHost.Variables(Some(sum))),
                 Host.LoadBalancerVariables(LoadBalancerHost.Variables(true, true))
             ],
             Network.Variables({ sent, sent2, sent3, sent4 })
         )];
-        assert ClientHost.ReceiveResponse(c.hosts[0].client, behavior[4].hosts[0].client, behavior[5].hosts[0].client, NoOp, msgOps);
-        assert NextStep(c, behavior[4], behavior[5], NoOp, HostActionStep(0, msgOps));
-        assert Next(c, behavior[4], behavior[5], NoOp);
+        assert ClientHost.ReceiveResponse(c.hosts[0].client, behavior[4].hosts[0].client, behavior[5].hosts[0].client, ReceiveResponse, msgOps);
+        assert NextStep(c, behavior[4], behavior[5], ReceiveResponse, HostActionStep(0, msgOps));
+        assert Next(c, behavior[4], behavior[5], ReceiveResponse);
     }
 }
